QED

code/ecdsap256sha2/Hacl.Impl.LowLevel.fst
@@ -1197,72 +1197,110 @@ let sq3 f f4 result memory tempBuffer =
   c3 +! h_3 +! c4
 
 
-#reset-options "--z3rlimit 1000"
-val sq: f: felem -> r: felem -> out: widefelem
-  -> Stack unit
-    (requires fun h -> live h out /\ live h f /\ live h r)
-    (ensures  fun h0 _ h1 -> modifies (loc out) h0 h1 /\ wide_as_nat h1 out = as_nat h0 r * as_nat h0 f)
+#reset-options "--z3rlimit 300"
+val sq: f: felem -> out: widefelem -> Stack unit
+    (requires fun h -> live h out /\ live h f /\ eq_or_disjoint f out)
+    (ensures  fun h0 _ h1 -> modifies (loc out) h0 h1 /\ wide_as_nat h1 out = as_nat h0 f * as_nat h0 f)
       
-let sq f r out =
+let sq f out =
   push_frame();
+      assert_norm (pow2 64 * pow2 64 * pow2 64 * pow2 64 = pow2 256);
 
-  let temp = create (size 8) (u64 0) in 
-  let tb = create (size 5) (u64 0) in 
-  let memory = create (size 12) (u64 0) in 
+  let wb = create (size 25) (u64 0) in 
+  
+  let temp = sub wb (size 0) (size 8) in 
+  let tb = sub wb (size 8) (size 5) in 
+  let memory = sub wb (size 13) (size 12) in 
    
   let f0 = f.(0ul) in
   let f1 = f.(1ul) in
   let f2 = f.(2ul) in
   let f3 = f.(3ul) in
-
-    let h0 = ST.get() in 
-  let b0 = sub temp (size 0) (size 4) in 
-  let c0 = sq0 r b0 memory tb in 
-    upd temp (size 4) c0;
-
-
-    let h1 = ST.get() in 
-    let bk0 = sub temp (size 0) (size 1) in 
-  let b1 = sub temp (size 1) (size 4) in   
-  let c1 = sq1 r b1 b1 memory tb in 
-      upd temp (size 5) c1; 
-
-
-    let h2 = ST.get() in
-      assert(Lib.Sequence.index (as_seq h1 bk0) 0 == Lib.Sequence.index (as_seq h1 temp) 0);
-  let bk1 = sub temp (size 0) (size 2) in 
-  let b2 = sub temp (size 2) (size 4) in 
-  let c2 = sq2 r b2 b2 memory tb in 
-    upd temp (size 6) c2;
+  let b0 = sub temp (size 0) (size 4) in
     
-  let h3 = ST.get() in 
+    let h0 = ST.get() in
+  let c0 = sq0 f b0 memory tb in 
+ 
+    upd temp (size 4) c0;
+    let h1 = ST.get() in
+
+    let bk0 = sub temp (size 0) (size 1) in 
+    assert(Lib.Sequence.index (as_seq h1 bk0) 0 == Lib.Sequence.index (as_seq h1 temp) 0); 
+
+  let b1 = sub temp (size 1) (size 4) in
+  let c1 = sq1 f b1 b1 memory tb in 
+    upd temp (size 5) c1; 
+    let h2 = ST.get() in 
+    
+    let bk1 = sub temp (size 0) (size 2) in 
     assert(Lib.Sequence.index (as_seq h2 bk1) 0 == Lib.Sequence.index (as_seq h2 temp) 0);
     assert(Lib.Sequence.index (as_seq h2 bk1) 1 == Lib.Sequence.index (as_seq h2 temp) 1);
-    assert_norm (pow2 64 * pow2 64 * pow2 64 * pow2 64 = pow2 256);
+
+  let b2 = sub temp (size 2) (size 4) in 
+  let c2 = sq2 f b2 b2 memory tb in 
+    upd temp (size 6) c2;
+
+    let h3 = ST.get() in 
      let bk2 = sub temp (size 0) (size 3) in 
-  let b3 = sub temp (size 3) (size 4) in 
-  let c3 = sq3 r b3 b3 memory tb in 
-    upd temp (size 7) c3;
-  admit();
-
-
+     
     assert(Lib.Sequence.index (as_seq h3 bk2) 0 == Lib.Sequence.index (as_seq h3 temp) 0);
     assert(Lib.Sequence.index (as_seq h3 bk2) 1 == Lib.Sequence.index (as_seq h3 temp) 1);
     assert(Lib.Sequence.index (as_seq h3 bk2) 2 == Lib.Sequence.index (as_seq h3 temp) 2);
 
-  assert_by_tactic (as_nat h0 r * (uint_v f2 * pow2 64 * pow2 64) == as_nat h0 r * uint_v f2 * pow2 64 * pow2 64) canon;
-  assert_by_tactic (as_nat h0 r * (uint_v f0) == as_nat h0 r * uint_v f0) canon;
-  assert_by_tactic (as_nat h0 r * (uint_v f1 * pow2 64) == as_nat h0 r * uint_v f1 * pow2 64) canon;
-  assert_by_tactic (as_nat h0 r * (uint_v f3 * pow2 64 * pow2 64 * pow2 64) == as_nat h0 r * uint_v f3 * pow2 64 * pow2 64 * pow2 64) canon;
+  let b3 = sub temp (size 3) (size 4) in 
+  let c3 = sq3 f b3 b3 memory tb in 
+    upd temp (size 7) c3;
 
-  dist_lemma_0 (as_nat h0 r) (uint_v f2 * pow2 64 * pow2 64) (uint_v f1 * pow2 64) (uint_v f0) (uint_v f3 * pow2 64 * pow2 64 * pow2 64);
+    let h4 = ST.get() in 
+
+ assert(
+    uint_v f0 * as_nat h0 f + 
+    uint_v f1 * as_nat h0 f * pow2 64 + 
+    uint_v f2 * as_nat h0 f * pow2 64 * pow2 64 + 
+    uint_v f3 * as_nat h0 f * pow2 64 * pow2 64 * pow2 64 = 
+    
+
+    as_nat h4 b3  * pow2 64 * pow2 64 * pow2 64 + 
+    uint_v (Lib.Sequence.index (as_seq h4 temp) 7) * pow2 64 * pow2 64 * pow2 64 * pow2 64  * pow2 64 * pow2 64 * pow2 64 +
+    uint_v (Lib.Sequence.index (as_seq h4 temp) 2) * pow2 64 * pow2 64 + 
+    uint_v (Lib.Sequence.index (as_seq h4 temp) 1) * pow2 64 + 
+    uint_v (Lib.Sequence.index (as_seq h4 temp) 0));
+
+
+    calc (==) {
+    as_nat h4 b3  * pow2 64 * pow2 64 * pow2 64 + 
+    uint_v (Lib.Sequence.index (as_seq h4 temp) 7) * pow2 64 * pow2 64 * pow2 64 * pow2 64  * pow2 64 * pow2 64 * pow2 64 +
+    uint_v (Lib.Sequence.index (as_seq h4 temp) 2) * pow2 64 * pow2 64 + 
+    uint_v (Lib.Sequence.index (as_seq h4 temp) 1) * pow2 64 + 
+    uint_v (Lib.Sequence.index (as_seq h4 temp) 0);
+    (==) {}
+    wide_as_nat h4 temp;};
+
+  calc (==)
+    {
+
+    as_nat h0 f * as_nat h0 f;
+    (==) {assert_by_tactic (
+    uint_v f0 * as_nat h0 f + 
+    uint_v f1 * as_nat h0 f * pow2 64 + 
+    uint_v f2 * as_nat h0 f * pow2 64 * pow2 64 + 
+    uint_v f3 * as_nat h0 f * pow2 64 * pow2 64 * pow2 64 == as_nat h0 f * (uint_v f0 + uint_v f1 * pow2 64 + uint_v f2 * pow2 64 * pow2 64 + uint_v f3 * pow2 64 * pow2 64 * pow2 64)) canon}
+
+    uint_v f0 * as_nat h0 f + 
+    uint_v f1 * as_nat h0 f * pow2 64 + 
+    uint_v f2 * as_nat h0 f * pow2 64 * pow2 64 + 
+    uint_v f3 * as_nat h0 f * pow2 64 * pow2 64 * pow2 64;
+    };
+
 
   copy out temp; 
-  
+    let h5 = ST.get() in 
+    assert(modifies (loc wb) h0 h4);
+    assert(modifies (loc out) h4 h5);
   pop_frame()
 
 
-val cmovznz4: cin: uint64 -> x: felem -> y: felem -> result: felem ->
+ val cmovznz4: cin: uint64 -> x: felem -> y: felem -> result: felem ->
   Stack unit
     (requires fun h -> live h x /\ live h y /\ live h result /\ disjoint x result /\ eq_or_disjoint y result)
     (ensures fun h0 _ h1 -> modifies1 result h0 h1 /\ 
